\documentclass{article}
\usepackage[english]{babel}
\usepackage{amsmath}

%%%%%%%%%% Start TeXmacs macros
\newcommand{\cdummy}{\cdot}
\newcommand{\tmaffiliation}[1]{\thanks{\textit{Affiliation:} #1}}
\newcommand{\tmop}[1]{\ensuremath{\operatorname{#1}}}
%%%%%%%%%% End TeXmacs macros

\begin{document}

\title{Back Propogation Explanation}

\author{
  Xing Chao
  \tmaffiliation{xingnix@live.com}
}

\maketitle

\section{Scalar $f$ , $w$ and $x$}

\subsection{Single layer}

\begin{eqnarray*}
  o & = & f ( w x-b )\\
  \frac{d o}{d w} & = & f' \frac{d }{d w} ( w x )\\
  & = & f' x\\
  e & = & \frac{1}{2} ( t-o )^{2}\\
  \frac{d e}{d w} & = & ( o-t ) \frac{\tmop{do}}{d w}\\
  & = & ( o-t ) f' x\\
  \Delta w & = & - \eta \frac{d e}{d w}\\
  & = & - \eta ( o-t ) f' x
\end{eqnarray*}

\subsection{Double layers}

\begin{eqnarray*}
  o^{( 2 )} & = & f_{2} ( w^{( 2 )} o^{( 1 )} -b_{}^{( 2 )} )\\
  o^{( 1 )} & = & f_{1} ( w^{( 1 )} x-b^{( 1 )} )\\
  e & = & \frac{1}{2} ( t-o^{( 2 )} )^{2}\\
  \frac{\partial e}{\partial w^{( 1 )}} & = & \frac{\partial e}{\partial o^{(
  2 )}} \cdummy \frac{\partial o^{( 2 )}}{\partial o^{( 1 )}} \cdummy
  \frac{\partial o^{( 1 )}}{\partial w^{( 1 )}}\\
  & = & ( o^{( 2 )} -t ) f_{2}' w^{( 2 )} f_{1}' x\\
  \Delta w^{( 1 )} & = & - \eta \frac{\partial e}{\partial w^{( 1 )}}\\
  & = & - \eta ( o^{( 2 )} -t ) f_{2}' w^{( 2 )} f_{1}' x
\end{eqnarray*}
let
\begin{eqnarray*}
  \delta^{( 2 )} & = & ( o^{( 2 )} -t ) f'_{2}\\
  \delta^{( 1 )} & = & \delta^{( 2 )} w^{( 2 )} f'_{1}
\end{eqnarray*}
then
\begin{eqnarray*}
  \Delta w^{( 1 )} & = & - \eta \delta^{( 1 )} x
\end{eqnarray*}

\subsection{Multi layers}

\begin{eqnarray*}
  o^{( i )} & = & f_{i} ( w^{( i )} o^{( i-1 )} -b_{}^{( i )} )\\
  e & = & \frac{1}{2} ( t-o^{( n )} )^{2}\\
  \frac{\partial e}{\partial w^{( i )}} & = & \dfrac{\partial e}{\partial o^{(
  n )}} \cdummy \frac{\partial o^{( n )}}{\partial o^{( n-1 )}} \cdots
  \frac{\partial o^{( i )}}{\partial w^{( i )}}\\
  & = & ( o^{( n )} -t ) f'_{n} \left[ \prod_{k=i+1}^{n} w^{( k )} f'_{k-1}
  \right] o^{( i-1 )}\\
  \Delta w^{( i )} & = & - \eta \frac{\partial e}{\partial w^{( i )}}\\
  & = & - \eta ( o^{( n )} -t ) f_{n}' \left[ \prod_{k=i+1}^{n} w^{( k )}
  \cdummy f_{k-1}' \right] \cdummy o^{( i-1 )}
\end{eqnarray*}
let
\begin{eqnarray*}
  \delta^{( n )} & = & 2 ( o^{( n )} -t ) f'_{n}\\
  \delta^{( k )} & = & \delta^{( k+1 )} w^{( k+1 )} f'_{k}
\end{eqnarray*}
then
\begin{eqnarray*}
  \Delta w^{( i )} & = & - \eta \delta^{( k )} o^{( i-1 )}
\end{eqnarray*}

\section{Multi nodes}

\subsection{Matrix $W$ , vector $X,O$ and $F$}

\begin{eqnarray*}
  O^{( i )} & = & F_{i} ( W^{( i )} O^{( i-1 )} )\\
  e & = & \frac{1}{2} ( T-O^{( n )} )^{T} ( T-O^{( n )} )\\
  \Delta e & = & \dfrac{\partial e}{\partial O^{( n )}} \cdummy \frac{\partial
  O^{( n )}}{\partial O^{( n-1 )}} \cdots \frac{\partial O^{( i+1 )}}{\partial
  O^{( i )}} \Delta O^{( i )}\\
  \Delta O^{( i )} & = & \tmop{diag} ( F'_{i} ) \Delta W^{( i )} O^{( i-1 )}\\
  \Delta e & = & ( O^{( n )} -T )^{T} \tmop{diag} ( F'_{n} ) \left[
  \prod^{n}_{k=i+1} W^{( k )} \cdummy \tmop{diag} ( F'_{k-1} ) \right] \Delta
  W^{( i )} O^{( i-1 )}\\
  \frac{\partial e}{\partial W^{( i )}} & = & \left[ \prod^{n}_{k=i+1}
  \tmop{diag} ( F'_{k-1} ) [ W^{( k )} ]^{T} \right] \tmop{diag} ( F'_{n} ) (
  O^{( n )} -T ) [ O^{( i-1 )} ]^{T}
\end{eqnarray*}
where
\begin{eqnarray*}
  F_{i} ( X ) & = & F_{i} \left( \left(\begin{array}{cccc}
    x_{1} & x_{2} & \cdots & x_{_{n}}
  \end{array}\right)^{T} \right)\\
  & = & \left(\begin{array}{cccc}
    f_{i} ( x_{1} ) & f_{i} ( x_{2} ) & \cdots & f_{i} ( x_{_{n}} )
  \end{array}\right)^{T}\\
  \frac{\partial}{\partial X} F_{i} ( X ) & = & \left(\begin{array}{cccc}
    f'_{i} ( x_{1} ) &  &  & \\
    & f'_{i} ( x_{2} ) &  & \\
    &  & \ddots & \\
    &  &  & f'_{i} ( x_{2} )
  \end{array}\right)\\
  & = & \tmop{diag} ( F'_{i} )
\end{eqnarray*}
let
\begin{eqnarray*}
  \delta^{( n )} & = & \tmop{diag} ( F'_{n} ) \cdummy 2 ( O^{( n )} -T )\\
  \delta^{( k )} & = & \tmop{diag} ( F'_{k} ) [ W^{( k+1 )} ]^{T} \cdummy
  \delta^{( k+1 )}
\end{eqnarray*}
then
\begin{eqnarray*}
  \Delta W^{( i )} & = & - \eta \delta^{( i )} [ O^{( i-1 )} ]^{T}
\end{eqnarray*}

\subsection{Summation notation}

Output of the j'th unit in the i'th layer:
\begin{eqnarray*}
  o_{j}^{( i )} & = & f_{i,j} ( y^{( i )}_{j} )\\
  y^{( i )}_{j} & = & \sum^{K}_{k=1} w_{j,k}^{( i )} o_{k}^{( i-1 )} -b_{j}^{(
  i )}\\
  \dfrac{\partial y_{p}^{( i+1 )}}{\partial y_{_{j}}^{( i )}} & = &
  \frac{\partial y_{p}^{( i+1 )}}{\partial o_{j}^{( i )}} \cdummy
  \frac{\partial o_{j}^{( i )}}{\partial y_{j}^{( i )}}\\
  & = & w^{( i+1 )}_{p,j} \cdummy f_{i,j}'\\
  \frac{\partial y_{j}^{( i )}}{\partial w_{j,k}^{( i )}} & = & o^{( i-1
  )}_{k}
\end{eqnarray*}

\begin{eqnarray*}
  e & = & \frac{1}{2} \sum^{J}_{j=1} ( t_{j} -o_{j}^{( n )} )^{2}\\
  \dfrac{\partial e}{\partial y_{_{j}}^{( n )}} & = & \frac{\partial
  e}{\partial o_{j}^{( n )}} \cdummy \frac{\partial o_{j}^{( n )}}{\partial
  y_{j}^{( n )}}\\
  & = & ( o^{( n )}_{j} -t_{j} ) \cdummy f_{n,j}'\\
  \dfrac{\partial e}{\partial y_{_{j}}^{( i )}} & = & \dfrac{\partial
  e}{\partial o_{_{j}}^{( i )}} \cdummy \frac{\partial o_{j}^{( i )}}{\partial
  y_{j}^{( i )}}\\
  & = & \sum^{P}_{P=1} \dfrac{\partial e}{\partial o_{_{p}}^{( i+1 )}}
  \cdummy \dfrac{\partial o_{p}^{( i+1 )}}{\partial o_{_{j}}^{( i )}} \cdummy
  \frac{\partial o_{j}^{( i )}}{\partial y_{j}^{( i )}}\\
  & = & \sum^{P}_{P=1} \dfrac{\partial e}{\partial o_{_{p}}^{( i+1 )}}
  \cdummy \frac{\partial o^{( i+1 )}_{p}}{\partial y^{( i+1 )}_{p}} \cdummy
  \dfrac{\partial y_{p}^{( i+1 )}}{\partial o_{_{j}}^{( i )}} \cdummy
  \frac{\partial o_{j}^{( i )}}{\partial y_{j}^{( i )}}\\
  & = & \sum^{P}_{P=1} \dfrac{\partial e}{\partial y^{( i+1 )}_{p}} \cdummy
  \dfrac{\partial y_{p}^{( i+1 )}}{\partial y_{j}^{( i )}}\\
  & = & \sum^{P}_{p=1} \dfrac{\partial e}{\partial y_{_{p}}^{( i+1 )}}
  \cdummy w^{( i+1 )}_{p,j} f_{i,j}'\\
  \frac{\partial e}{\partial w^{( i )}_{j,k}} & = & \dfrac{\partial
  e}{\partial y_{_{j}}^{( i )}} \cdummy \frac{\partial y_{j}^{( i )}}{\partial
  w_{j,k}^{( i )}}\\
  & = & \dfrac{\partial e}{\partial y_{_{j}}^{( i )}} \cdummy o_{k}^{( i-1 )}
\end{eqnarray*}
let
\begin{eqnarray*}
  \delta_{j}^{( n )} & = & \dfrac{\partial e}{\partial y_{_{j}}^{( n )}}\\
  & = & ( o^{( n )}_{j} -t_{j} ) \cdummy f_{n,j}'\\
  \delta_{j}^{( i )} & = & \dfrac{\partial e}{\partial y_{_{j}}^{( i )}}\\
  & = & \sum^{P}_{p=1} \delta^{( i+1 )}_{p} \cdummy w^{( i+1 )}_{p,j}
  f_{i,j}'
\end{eqnarray*}
then
\begin{eqnarray*}
  \Delta w_{j,k}^{( i )} & = & - \eta \frac{\partial e}{\partial w^{( i
  )}_{j,k}}\\
  & = & - \eta \delta^{( i )}_{j} o^{( i-1 )}_{k}
\end{eqnarray*}

\end{document}
